begin restructure

Common/Ctx.lean
@@ -1,29 +1,30 @@
 
-import Common.Term
-import Common.Term.Substitution
+import Common.Substitution
 
-abbrev Ctx := List Term
+variable {T : Type} [Inhabited T] [SubstitutionType T] [SubstitutionTypeLaws T]
+
+def Ctx (T : Type) := List T
 
 @[simp]
-def nth : List Term -> Nat -> Term
-| [], _ => .none
+def nth : List T -> Nat -> T
+| [], _ => default
 | .cons h _, 0 => h
 | .cons _ t, n + 1 => nth t n
 
 @[simp]
-def dnth : List Term -> Nat -> Term
-| [], _ => .none
+def dnth : List T -> Nat -> T
+| [], _ => default
 | .cons h _, 0 => [S]h
 | .cons _ t, n + 1 => [S](dnth t n)
 
 infix:1000 "@" => nth
 infix:1000 "d@" => dnth
 
-theorem dnth_as_nth : Γ d@ n = [Sn (n + 1)](Γ @ n) := by
-induction n generalizing Γ
-case zero =>
-  cases Γ <;> simp
-case succ n ih =>
-  simp; cases Γ <;> simp
-  case _ A Γ =>
-    rw [ih]; simp
+-- theorem dnth_as_nth : Γ d@ n = [Sn (n + 1)](Γ @ n) := by
+-- induction n generalizing Γ
+-- case zero =>
+--   cases Γ <;> simp
+-- case succ n ih =>
+--   simp; cases Γ <;> simp
+--   case _ A Γ =>
+--     rw [ih]; simp
