Common/Reduction.lean
@@ -1,5 +1,202 @@
+import Common.Substitution
 
-import Common.Reduction.Definition
-import Common.Reduction.Basic
-import Common.Reduction.Plus
-import Common.Reduction.Confluence
+class ReductionCompletion (T : Type) (R : T -> T -> Prop) where
+  compl : T -> T
+
+class ReductionTriangle (T : Type) (R : T -> T -> Prop) [ReductionCompletion T R] where
+  triangle : R t s -> R s (ReductionCompletion.compl R t)
+
+variable {T : Type} {R : T -> T -> Prop}
+
+inductive Star : T -> T -> Prop where
+| refl : Star t t
+| step : Star x y -> R y z -> Star x z
+
+inductive StarB : Nat -> T -> T -> Prop where
+| refl : StarB n t t
+| step : StarB n x y -> R y z -> StarB (n + 1) x z
+
+def ConvB (g1 g2 : Nat) (x y : T) : Prop :=
+  ∃ z, @StarB T R g1 x z ∧ @StarB T R g2 y z
+
+def Conv (x y : T) : Prop :=
+  ∃ z, @Star T R x z ∧ @Star T R y z
+
+namespace Star
+  theorem trans : @Star T R x y -> @Star T R y z -> @Star T R x z := by
+  intro r1 r2; induction r2 generalizing x
+  case _ => apply r1
+  case _ a b _ r2 ih => apply Star.step (ih r1) r2
+
+  theorem promote (Rprm : ∀ {x y}, R1 x y -> R2 x y) :
+    @Star T R1 x y -> @Star T R2 x y
+  := by
+  intro r; induction r
+  case _ => constructor
+  case _ _ r ih => constructor; apply ih; apply Rprm r
+end Star
+
+namespace StarB
+  @[simp]
+  def star (f : T -> T) : Nat -> T -> T
+  | 0, t => t
+  | n + 1, t => star f n (f t)
+
+  theorem weaken k : @StarB T R g x y -> @StarB T R (g + k) x y := by
+  intro r; induction r generalizing k
+  case _ => constructor
+  case _ n _ _ _ _ r2 ih =>
+    have lem : n + 1 + k = n + k + 1 := by omega
+    rw [lem]; apply StarB.step (ih k) r2
+
+  theorem trans : @StarB T R g1 x y -> @StarB T R g2 y z -> @StarB T R (g1 + g2) x z := by
+  intro r1 r2; induction r2 generalizing g1 x
+  case _ n t => apply weaken n r1
+  case _ n a b c _ r2 ih => apply StarB.step (ih r1) r2
+
+  theorem promote (Rprm : ∀ {x y}, R1 x y -> R2 x y) :
+    @StarB T R1 n x y -> @StarB T R2 n x y
+  := by
+  intro r; induction r
+  case _ => constructor
+  case _ _ r ih => constructor; apply ih; apply Rprm r
+
+  theorem star_sound n t : (∀ t, R t (f t)) -> @StarB T R n t (star f n t) := by
+  intro h
+  have lem : ∀ {t n}, R (star f n t) (star f n (f t)) := by
+    intro t n; induction n generalizing t; simp; apply h _
+    case _ n ih => simp; apply ih
+  induction n
+  case _ => simp; constructor
+  case _ n ih =>
+    constructor; apply ih; simp; apply lem
+end StarB
+
+namespace ConvB
+  @[simp]
+  def convb [BEq T] (f : T -> T) (g1 g2 : Nat) (a b : T) : Bool :=
+    StarB.star f g1 a == StarB.star f g2 b
+
+  theorem weaken k1 k2 : @ConvB T R g1 g2 x y -> @ConvB T R (g1 + k1) (g2 + k2) x y := by
+  intro h; cases h; case _ w h =>
+    exists w; apply And.intro
+    apply StarB.weaken k1 h.1; apply StarB.weaken k2 h.2
+
+  theorem promote (Rprm : ∀ {x y}, R1 x y -> R2 x y) :
+    @ConvB T R1 g1 g2 x y -> @ConvB T R2 g1 g2 x y
+  := by
+  intro h; cases h; case _ w h =>
+    exists w; apply And.intro
+    apply StarB.promote Rprm h.1; apply StarB.promote Rprm h.2
+
+  theorem conv_sound [BEq T] [LawfulBEq T] : (∀ t, R t (f t)) -> convb f g1 g2 a b -> @ConvB T R g1 g2 a b := by
+  intro h1 h2; simp at h2
+  have lem1 := StarB.star_sound g1 a h1
+  have lem2 := StarB.star_sound g2 b h1
+  exists (StarB.star f g1 a); apply And.intro
+  apply lem1; rw [h2]; apply lem2
+end ConvB
+
+namespace Star
+  variable [ReductionCompletion T R] [ReductionTriangle T R]
+
+  theorem strip : R s t1 -> @Star T R s t2 -> ∃ t, @Star T R t1 t ∧ R t2 t := by
+  intro h1 h2
+  induction h2 generalizing t1
+  case _ t' => exists t1; apply And.intro; apply Star.refl; apply h1
+  case _ n' x y z _r1 r2 ih =>
+    replace ih := ih h1
+    cases ih
+    case _ w ih =>
+      replace r2 := ReductionTriangle.triangle r2
+      have lem := ReductionTriangle.triangle ih.2
+      replace lem := Star.step ih.1 lem
+      exists (ReductionCompletion.compl R y)
+
+  theorem confluence : @Star T R s t1 -> @Star T R s t2 -> @Conv T R t1 t2 := by
+  intro h1 h2
+  induction h1 generalizing t2
+  case _ z =>
+    exists t2; apply And.intro
+    apply h2; apply Star.refl
+  case _ g3 s y t1 _r1 r2 ih =>
+    replace ih := ih h2
+    cases ih; case _ w ih =>
+      have lem := strip r2 ih.1
+      cases lem; case _ q lem =>
+        exists q; apply And.intro
+        apply lem.1; apply Star.step ih.2 lem.2
+end Star
+
+namespace StarB
+  variable [ReductionCompletion T R] [ReductionTriangle T R]
+
+  theorem strip : R s t1 -> @StarB T R n s t2 -> ∃ t, @StarB T R n t1 t ∧ R t2 t := by
+  intro h1 h2
+  induction h2 generalizing t1
+  case _ t' => exists t1; apply And.intro; apply StarB.refl; apply h1
+  case _ n' x y z _r1 r2 ih =>
+    replace ih := ih h1
+    cases ih
+    case _ w ih =>
+      replace r2 := ReductionTriangle.triangle r2
+      have lem := ReductionTriangle.triangle ih.2
+      replace lem := StarB.step ih.1 lem
+      exists (ReductionCompletion.compl R y)
+
+  theorem confluence : @StarB T R g1 s t1 -> @StarB T R g2 s t2 -> @ConvB T R g2 g1 t1 t2 := by
+  intro h1 h2
+  induction h1 generalizing t2
+  case _ z =>
+    exists t2; apply And.intro
+    apply h2; apply StarB.refl
+  case _ g3 s y t1 _r1 r2 ih =>
+    replace ih := ih h2
+    cases ih; case _ w ih =>
+      have lem := strip r2 ih.1
+      cases lem; case _ q lem =>
+        exists q; apply And.intro
+        apply lem.1; apply StarB.step ih.2 lem.2
+end StarB
+
+namespace Conv
+  theorem refl : @Conv T R t t := by
+  exists t; apply And.intro; apply Star.refl; apply Star.refl
+
+  theorem sym : @Conv T R x y -> @Conv T R y x := by
+  intro h; cases h; case _ w h =>
+    exists w; apply And.intro; apply h.2; apply h.1
+
+  theorem trans [ReductionCompletion T R] [ReductionTriangle T R] :
+    @Conv T R x y -> @Conv T R y z -> @Conv T R  x z
+  := by
+  intro h1 h2
+  cases h1; case _ w1 h1 =>
+  cases h2; case _ w2 h2 =>
+    have lem := Star.confluence h1.2 h2.1
+    cases lem; case _ q lem =>
+      exists q; apply And.intro
+      apply Star.trans h1.1 lem.1
+      apply Star.trans h2.2 lem.2
+end Conv
+
+namespace ConvB
+  theorem refl : @ConvB T R g1 g2 t t := by
+  exists t; apply And.intro; apply StarB.refl; apply StarB.refl
+
+  theorem sym : @ConvB T R g1 g2 x y -> @ConvB T R g2 g1 y x := by
+  intro h; cases h; case _ w h =>
+    exists w; apply And.intro; apply h.2; apply h.1
+
+  theorem trans [ReductionCompletion T R] [ReductionTriangle T R] :
+    @ConvB T R gx gy1 x y -> @ConvB T R gy2 gz y z -> @ConvB T R (gx + gy2) (gz + gy1) x z
+  := by
+  intro h1 h2
+  cases h1; case _ w1 h1 =>
+  cases h2; case _ w2 h2 =>
+    have lem := StarB.confluence h1.2 h2.1
+    cases lem; case _ q lem =>
+      exists q; apply And.intro
+      apply StarB.trans h1.1 lem.1
+      apply StarB.trans h2.2 lem.2
+end ConvB
