Fomega/Basic/Classification.lean
@@ -1,44 +1,46 @@
 import Common
 import Fomega.Proof
-import Fomega.PreProof
 import Fomega.Basic.Weaken
 import Fomega.Basic.Substitution
 
 namespace Fomega.Proof
 
   @[simp]
-  abbrev AllDestructLemmaType (Γ : Ctx) : (v : JudgmentVariant) -> JudgmentIndex v -> Prop
-  | .prf => λ (t, T) => ∀ A B K, t = .all mf A B -> T =β= .const K -> (A::Γ) ⊢ B : .const K
+  abbrev AllDestructLemmaType (Γ : Ctx Term) : (v : JudgmentVariant) -> JudgmentIndex v -> Prop
+  | .prf => λ (t, T) => ∀ A B K, t = Π[A] B -> T =β= .const K -> (A::Γ) ⊢ B : .const K
   | .wf => λ () => True
 
   theorem all_destruct_lemma : Judgment v Γ ix -> AllDestructLemmaType Γ v ix := by
   intro j; induction j <;> simp at *
   case pi K1 K2 _ j1 j2 _ _ =>
-    intro A B K h1 h2 T h3 h4
-    have lem := @RedConv.const_conv_implies_eq K2 K (by exists T); subst lem
-    subst h2; subst h1; apply j2
+    intro A B K h1 h2 h3; subst h2; subst h1
+    cases h3; case _ T r =>
+    have lem := Red.const_conv_implies_eq K2 K (by exists T); subst lem
+    apply j2
   case conv A' B' _ _ _ cv ih1 _ih2 =>
-    intro A B K h1 T h2 h3
-    have lem : A' =β= .const K := by apply RedConv.trans cv (by exists T)
+    intro A B K h1 h2
+    cases h2; case _ T h2 =>
+    have lem : A' =β= .const K := by apply Red.trans cv (by exists T)
     cases lem; case _ q r =>
-      apply ih1 _ _ _ h1 q r.1 r.2
+      apply ih1 _ _ _ h1 (by exists q)
 
   @[simp]
-  abbrev ProdDestructLemmaType (Γ : Ctx) : (v : JudgmentVariant) -> JudgmentIndex v -> Prop
+  abbrev TimesDestructLemmaType (Γ : Ctx Term) : (v : JudgmentVariant) -> JudgmentIndex v -> Prop
   | .prf => λ (t, T) => ∀ A B K, t = .times A B -> T =β= .const K -> Γ ⊢ A : ★ ∧ Γ ⊢ B : ★
   | .wf => λ () => True
 
-  theorem prod_destruct_lemma : Judgment v Γ ix -> ProdDestructLemmaType Γ v ix := by
+  theorem times_destruct_lemma : Judgment v Γ ix -> TimesDestructLemmaType Γ v ix := by
   intro j; induction j <;> simp at *
   case prod j1 j2 _ _ =>
-    intro A B K h1 h2 x r1 r2; subst h1; subst h2
-    have lem := @RedConv.const_conv_implies_eq K .type (by exists x)
-    subst lem; apply And.intro; apply j1; apply j2
+    intro A B K h1 h2 h3; subst h1; subst h2
+    cases h3; case _ T h3 =>
+      have lem := Red.const_conv_implies_eq .type K (by exists T)
+      subst lem; apply And.intro; apply j1; apply j2
   case conv A' B' _ _ _ cv ih1 _ih2 =>
-    intro A B K h1 T h2 h3
-    have lem : A' =β= .const K := by apply RedConv.trans cv (by exists T)
+    intro A B K h1 h2
+    have lem : A' =β= .const K := by apply Red.trans cv h2
     cases lem; case _ q r =>
-      apply ih1 _ _ _ h1 q r.1 r.2
+      apply ih1 _ _ _ h1 (by exists q)
 
   @[simp]
   abbrev class_idx (t A : Term) : JudgmentIndex v :=
@@ -47,30 +49,40 @@ namespace Fomega.Proof
     | .wf => ()
 
   @[simp]
-  abbrev ClassType (Γ : Ctx) : (v : JudgmentVariant) -> JudgmentIndex v -> Prop
+  abbrev ClassType (Γ : Ctx Term) : (v : JudgmentVariant) -> JudgmentIndex v -> Prop
   | .prf => λ (_, A) => A = □ ∨ (∃ K, Γ ⊢ A : .const K)
-  | .wf => λ () => True
+  | .wf => λ () => ∀ x, ∃ K, Γ ⊢ Γ d@ x : .const K
 
   theorem classification_lemma : Judgment v Γ ix -> ClassType Γ v ix := by
   intro j; induction j <;> simp at *
-  case var K _ j1 j2 _ih =>
-    apply Or.inr; exists K; rw [j2]; apply j1
+  case nil =>
+    unfold default; unfold instInhabited_Term; simp
+    exists .kind; constructor; constructor
+  case cons A K j1 j2 ih1 _ =>
+    intro x; cases x <;> simp at *
+    case _ =>
+      exists K; have lem := weaken j2 j2; simp at lem
+      apply lem
+    case _ x =>
+      replace ih1 := ih1 x; cases ih1; case _ K ih1 =>
+        exists K; have lem := weaken j2 ih1; simp at lem
+        apply lem
+  case var Γ _ x j1 j2 ih =>
+    subst j2; apply Or.inr; apply ih x
   case pi K1 K2 _ j1 _ ih1 ih2 =>
     cases ih1
     case _ h =>
-      cases K2; simp at *; exists .kind
+      cases K2; simp at *; apply Or.inr; exists .kind
       constructor; apply judgment_ctx_wf j1
-      simp
     case _ h =>
-      cases K2; simp at *; exists .kind
+      cases K2; simp at *; apply Or.inr; exists .kind
       constructor; apply judgment_ctx_wf j1
-      simp
   case lam K1 K2 _ _ j1 j2 j3 _ _ _ =>
     exists K2; constructor; apply j1; apply j2
   case app Γ f A B a B' j1 j2 j3 _ ih2 =>
     cases ih2; case _ K ih2 =>
       have lem := all_destruct_lemma ih2; simp at lem
-      replace lem := lem A B K rfl rfl (.const K) Red.refl Red.refl
+      replace lem := lem A B K rfl rfl Red.refl
       replace lem := Proof.beta lem j2; simp at lem
       apply Or.inr; exists K
       rw [j3]; apply lem
@@ -78,13 +90,13 @@ namespace Fomega.Proof
   case pair j1 j2 _ _ _ _=> exists .type; constructor; apply j1; apply j2
   case fst t A B j ih =>
     cases ih; case _ K ih =>
-      have lem := prod_destruct_lemma ih; simp at lem
-      replace lem := lem A B K rfl rfl (.const K) Red.refl Red.refl
+      have lem := times_destruct_lemma ih; simp at lem
+      replace lem := lem A B K rfl rfl Red.refl
       apply Or.inr; exists .type; apply lem.1
   case snd t A B j ih =>
     cases ih; case _ K ih =>
-      have lem := prod_destruct_lemma ih; simp at lem
-      replace lem := lem A B K rfl rfl (.const K) Red.refl Red.refl
+      have lem := times_destruct_lemma ih; simp at lem
+      replace lem := lem A B K rfl rfl Red.refl
       apply Or.inr; exists .type; apply lem.2
   case unit j _ => exists .type; constructor; apply j
   case unit_ty j _ => exists .kind; constructor; apply j
