Fomega/Basic/Preservation.lean
@@ -1,37 +1,33 @@
 import Common
 import Fomega.Proof
-import Fomega.PreProof
 import Fomega.Basic.Weaken
 import Fomega.Basic.Substitution
-import Fomega.Basic.Inversion
 import Fomega.Basic.Classification
 
 namespace Fomega.Proof
 
   @[simp]
-  abbrev LamDestructLemmaType (Γ : Ctx) : (v : JudgmentVariant) -> JudgmentIndex v -> Prop
-  | .prf => λ (t, T) => ∀ m C A b B, t = .lam m C b -> T =β= .all mf A B ->
-    m = mf
-    ∧ (∃ K, A =β= C ∧ Γ ⊢ C : .const K)
-    ∧ (∃ K D, B =β= D ∧ (C::Γ) ⊢ D : .const K ∧ (C::Γ) ⊢ b : D)
+  abbrev LamDestructLemmaType (Γ : Ctx Term) : (v : JudgmentVariant) -> JudgmentIndex v -> Prop
+  | .prf => λ (t, T) => ∀ A b B, t = `λ b -> T =β= Π[A] B ->
+    ∃ C, ((∃ K, A =β= C ∧ Γ ⊢ C : .const K)
+    ∧ (∃ K D, B =β= D ∧ (C::Γ) ⊢ D : .const K ∧ (C::Γ) ⊢ b : D))
   | .wf => λ () => True
 
   theorem lam_destruct_lemma : Judgment v Γ ix -> LamDestructLemmaType Γ v ix := by
   intro j; induction j <;> simp at *
   case lam A' K1 K2 B' t j1 j2 j3 _ _ _ =>
-    intro m C A b B h1 h2 h3 x r1 r2; subst h1; subst h2; subst h3
-    have lem := @RedConv.all_congr _ A B _ A' B' (by exists x)
-    simp; apply And.intro; apply And.intro; apply lem.2.1
+    intro A b B h1 h2; subst h1
+    have lem := Red.all_congr h2; exists A'
+    apply And.intro; apply And.intro; apply Red.sym lem.1
     exists (dom K1 K2); exists K2; exists B'; apply And.intro
-    apply lem.2.2; apply And.intro; apply j2; apply j3
+    apply Red.sym lem.2; apply And.intro; apply j2; apply j3
   case conv A' B' _ _ _ cv ih1 _ih2 =>
-    intro m C A b B h1 x r1 r2; cases cv; case _ w r3 =>
-      have lem := Red.confluence r1 r3.2
-      cases lem; case _ q r4 =>
-        apply ih1 m C A b B h1 q (Red.trans r3.1 r4.2) (Red.trans r2 r4.1)
+    intro A b B h1 h2; subst h1
+    have lem := Red.trans cv h2
+    apply ih1 A b B rfl lem
 
   @[simp]
-  abbrev PairDestructLemmaType (Γ : Ctx) : (v : JudgmentVariant) -> JudgmentIndex v -> Prop
+  abbrev PairDestructLemmaType (Γ : Ctx Term) : (v : JudgmentVariant) -> JudgmentIndex v -> Prop
   | .prf => λ (t, T) => ∀ c d A B, t = .pair c d -> T =β= .times A B ->
     (∃ C, A =β= C ∧ Γ ⊢ c : C ∧ Γ ⊢ C : ★)
     ∧ (∃ D, B =β= D ∧ Γ ⊢ d : D ∧ Γ ⊢ D : ★)
@@ -40,19 +36,18 @@ namespace Fomega.Proof
   theorem pair_destruct_lemma : Judgment v Γ ix -> PairDestructLemmaType Γ v ix := by
   intro j; induction j <;> simp at *
   case pair Γ a A b B j1 j2 j3 j4 _ _ _ _ =>
-    intro c d A' B' h1 h2 x r1 r2; subst h1; subst h2
-    have lem := @RedConv.times_congr A' B' A B (by exists x)
-    apply And.intro; exists A; apply And.intro; apply lem.1
+    intro c d A' B' h1 h2 h3; subst h1; subst h2
+    have lem := Red.times_congr h3
+    apply And.intro; exists A; apply And.intro; apply Red.sym lem.1
     apply And.intro; apply j1; apply j3
-    exists B; apply And.intro; apply lem.2
+    exists B; apply And.intro; apply Red.sym lem.2
     apply And.intro; apply j2; apply j4
   case conv A' B' _ _ _ cv ih1 _ih2 =>
-    intro c d A B h1 x r1 r2; cases cv; case _ w r3 =>
-      have lem := Red.confluence r1 r3.2
-      cases lem; case _ q r4 =>
-        apply ih1 c d A B h1 q (Red.trans r3.1 r4.2) (Red.trans r2 r4.1)
+    intro c d A B h1 h2; subst h1
+    have lem := Red.trans cv h2
+    apply ih1 c d A B rfl lem
 
-  inductive CtxRed : Ctx -> Ctx -> Prop where
+  inductive CtxRed : Ctx Term -> Ctx Term -> Prop where
   | nil : CtxRed [] []
   | head : A -β> A' -> CtxRed Γ Γ' -> CtxRed (A::Γ) (A'::Γ')
   | tail : CtxRed Γ Γ' -> CtxRed (A::Γ) (A::Γ')
@@ -67,25 +62,21 @@ namespace Fomega.Proof
     intro j; induction j generalizing x; simp
     case _ A A' Γ Γ' r1 _r2 ih =>
       cases x <;> simp
-      case _ => apply Or.inr; apply Red.subst1_same; apply r1
+      case _ => apply Or.inr; apply Red.red1_subst_same; apply r1
       case _ x =>
         cases (ih x)
         case _ ih => rw [ih]; apply Or.inl rfl
-        case _ ih => apply Or.inr; apply Red.subst1_same; apply ih
+        case _ ih => apply Or.inr; apply Red.red1_subst_same; apply ih
     case _ Γ Γ' A _ ih =>
       cases x <;> simp
       case _ x =>
         cases (ih x)
         case _ h => apply Or.inl; rw [h]
-        case _ h => apply Or.inr; apply Red.subst1_same; apply h
+        case _ h => apply Or.inr; apply Red.red1_subst_same; apply h
   end CtxRed
 
-  inductive CtxRedStar : Ctx -> Ctx -> Prop where
-  | refl : CtxRedStar t t
-  | step : CtxRed x y -> CtxRedStar y z -> CtxRedStar x z
-
   @[simp]
-  abbrev Preservation1Type (Γ : Ctx) : (v : JudgmentVariant) -> JudgmentIndex v -> Prop
+  abbrev Preservation1Type (Γ : Ctx Term) : (v : JudgmentVariant) -> JudgmentIndex v -> Prop
   | .prf => λ (t, A) => ∀ {t' Γ'}, t = t' ∨ t -β> t' -> CtxRed Γ Γ' -> Γ' ⊢ t' : A
   | .wf => λ () => ∀ {Γ'}, CtxRed Γ Γ' -> ⊢ Γ'
 
@@ -104,20 +95,20 @@ namespace Fomega.Proof
     cases r1
     case _ r1 => rw [<-r1]; constructor; apply ih r2
     case _ r1 => cases r1
-  case var Γ x K T j1 j2 ih =>
-    intro t' Γ' r1 r2
-    cases r1
-    case _ r1 =>
-      rw [<-r1]; have lem := CtxRed.nth x r2
-      apply @Judgment.conv _ _ (Γ' d@ x) _ K
-      constructor; apply ih lem r2; rfl
-      rw [j2]; apply ih (Or.inl rfl) r2
-      rw [j2]; cases lem
-      case _ h2 => rw [h2]; apply RedConv.refl
-      case _ h2 =>
-        exists (Γ' d@ x); apply And.intro
-        apply RedStar.refl; apply Red.trans_flip RedStar.refl h2
-    case _ r1 => cases r1
+  case var => sorry
+    -- intro t' Γ' r1 r2
+    -- cases r1
+    -- case _ r1 =>
+    --   rw [<-r1]; have lem := CtxRed.nth x r2
+    --   apply @Judgment.conv _ _ (Γ' d@ x) _ K
+    --   constructor; apply ih lem r2; rfl
+    --   rw [j2]; apply ih (Or.inl rfl) r2
+    --   rw [j2]; cases lem
+    --   case _ h2 => rw [h2]; apply RedConv.refl
+    --   case _ h2 =>
+    --     exists (Γ' d@ x); apply And.intro
+    --     apply RedStar.refl; apply Red.trans_flip RedStar.refl h2
+    -- case _ r1 => cases r1
   case pi Γ A K1 K2 B j1 j2 ih1 ih2 =>
     intro t' Γ' r1 r2
     cases r1
@@ -142,16 +133,6 @@ namespace Fomega.Proof
       apply ih3 (Or.inl rfl) (.tail r2)
     case _ r1 =>
       cases r1
-      case _ A' r1 =>
-        apply @Judgment.conv _ _ (.all mf A' B) _ K2
-        constructor; apply ih1 (Or.inr r1) r2
-        apply ih2 (Or.inl rfl) (.head r1 r2)
-        apply ih3 (Or.inl rfl) (.head r1 r2)
-        constructor; apply ih1 (Or.inl rfl) r2
-        apply ih2 (Or.inl rfl) (.tail r2)
-        exists (.all mf A' B); apply And.intro
-        apply Red.refl; apply Red.trans_flip Red.refl
-        apply Red.all_congr1 r1
       case _ t' r1 =>
         constructor; apply ih1 (Or.inl rfl) r2
         apply ih2 (Or.inl rfl) (.tail r2)
@@ -164,29 +145,27 @@ namespace Fomega.Proof
       apply ih2 (Or.inl rfl) r2; apply j3
     case _ r1 =>
       cases r1
-      case _ m2 A' b =>
+      case _ A' b =>
         replace ih1 := ih1 (Or.inl rfl) r2
         replace ih2 := ih2 (Or.inl rfl) r2
         have lem := lam_destruct_lemma ih1; simp at lem
-        replace lem := lem m2 A' A b B rfl rfl rfl (.all mf A B) Red.refl Red.refl
-        cases lem.2.1.2; case _ K1 lem2 =>
-        cases lem.2.2; case _ K2 lem3 =>
+        replace lem := lem A b B rfl Red.refl
+        cases lem; case _ A' lem =>
+        cases lem.1.2; case _ K1 lem2 =>
+        cases lem.2; case _ k2 lem3 =>
         cases lem3; case _ D lem3 =>
           have ih2' : Γ' ⊢ a : A' := by
             apply Judgment.conv; apply ih2
-            apply lem2; apply lem.2.1.1
+            apply lem2; apply lem.1.1
           have lem4 := Proof.beta lem3.2.2 ih2'; simp at *; rw [j3]
           have lem5 := classification ih1
           cases lem5 <;> simp at *; case _ lem5 =>
           cases lem5; case _ K3 lem5 =>
             have lem6 := all_destruct_lemma lem5; simp at lem6
-            replace lem6 := lem6 A B K3 rfl rfl (.const K3) Red.refl Red.refl
+            replace lem6 := lem6 A B K3 rfl rfl Red.refl
             replace lem6 := Proof.beta lem6 ih2; simp at lem6
             apply Judgment.conv; apply lem4; apply lem6
-            apply RedConv.subst; apply RedConv.sym; apply lem3.1
-      case _ =>
-        have lem := IsPreProof.from_proof j1; simp at lem
-        cases lem
+            apply Red.subst_same; apply Red.sym; apply lem3.1
       case _ f' r1 =>
         constructor; apply ih1 (Or.inr r1) r2
         apply ih2 (Or.inl rfl) r2; apply j3
@@ -197,17 +176,18 @@ namespace Fomega.Proof
         cases lem1 <;> simp at *; case _ lem1 =>
           cases lem1; case _ K lem1 =>
             have lem2 := all_destruct_lemma lem1; simp at lem2
-            replace lem2 := lem2 A B K rfl rfl (.const K) Red.refl Red.refl
+            replace lem2 := lem2 A B K rfl rfl Red.refl
             have lem3 := Proof.beta lem2 j2; simp at lem3
             apply @Judgment.conv _ _ (B β[a']) _ K
             constructor; apply j1; apply ih2 (Or.inr r1) r2; rfl
             rw [j3]; apply lem3; rw [j3]; simp
-            apply RedConv.subst2
-            intro n t h1; cases n <;> simp at *; subst h1
-            exists a'; apply And.intro
-            apply Red.refl; apply Red.trans_flip Red.refl r1
-            intro n k h1; cases n <;> simp at *; apply h1
-            apply RedConv.refl
+            sorry
+            -- apply RedConv.subst2
+            -- intro n t h1; cases n <;> simp at *; subst h1
+            -- exists a'; apply And.intro
+            -- apply Red.refl; apply Red.trans_flip Red.refl r1
+            -- intro n k h1; cases n <;> simp at *; apply h1
+            -- apply RedConv.refl
   case prod Γ A B j1 j2 ih1 ih2 =>
     intro t' Γ' r1 r2
     cases r1
@@ -239,19 +219,17 @@ namespace Fomega.Proof
     case _ r1 => rw [<-r1]; constructor; apply ih (Or.inl rfl) r2
     case _ r1 =>
       cases r1
-      case _ => have lem := IsPreProof.from_proof j; cases lem
       case _ s =>
         replace ih := ih (Or.inl rfl) r2
         have lem := pair_destruct_lemma ih; simp at lem
-        replace lem := lem t' s A B rfl rfl (.times A B) Red.refl Red.refl
+        replace lem := lem t' s A B rfl rfl Red.refl
         have lem2 := classification ih; simp at lem2
         cases lem2; case _ K lem2 =>
         cases lem.1; case _ C lem =>
-          replace lem2 := prod_destruct_lemma lem2; simp at lem2
-          replace lem2 := lem2 A B K rfl rfl (.const K) Red.refl Red.refl
+          replace lem2 := times_destruct_lemma lem2; simp at lem2
+          replace lem2 := lem2 A B K rfl rfl Red.refl
           apply Judgment.conv; apply lem.2.1; apply lem2.1
-          apply RedConv.sym; apply lem.1
-      case _ => have lem := IsPreProof.from_proof j; cases lem
+          apply Red.sym; apply lem.1
       case _ t' r1 => constructor; apply ih (Or.inr r1) r2
   case snd Γ t A B j ih =>
     intro t' Γ' r1 r2
@@ -259,19 +237,17 @@ namespace Fomega.Proof
     case _ r1 => rw [<-r1]; constructor; apply ih (Or.inl rfl) r2
     case _ r1 =>
       cases r1
-      case _ => have lem := IsPreProof.from_proof j; cases lem
       case _ s =>
         replace ih := ih (Or.inl rfl) r2
         have lem := pair_destruct_lemma ih; simp at lem
-        replace lem := lem s t' A B rfl rfl (.times A B) Red.refl Red.refl
+        replace lem := lem s t' A B rfl rfl Red.refl
         have lem2 := classification ih; simp at lem2
         cases lem2; case _ K lem2 =>
         cases lem.2; case _ C lem =>
-          replace lem2 := prod_destruct_lemma lem2; simp at lem2
-          replace lem2 := lem2 A B K rfl rfl (.const K) Red.refl Red.refl
+          replace lem2 := times_destruct_lemma lem2; simp at lem2
+          replace lem2 := lem2 A B K rfl rfl Red.refl
           apply Judgment.conv; apply lem.2.1; apply lem2.2
-          apply RedConv.sym; apply lem.1
-      case _ => have lem := IsPreProof.from_proof j; cases lem
+          apply Red.sym; apply lem.1
       case _ t' r1 => constructor; apply ih (Or.inr r1) r2
   case unit Γ j ih =>
     intro t' Γ' r1 r2
@@ -306,41 +282,35 @@ namespace Fomega.Proof
   theorem preservation_term : Γ ⊢ t : A -> t -β>* t' -> Γ ⊢ t' : A := by
   intro j r; induction r
   case _ => apply j
-  case _ r1 _r2 ih =>
-    have lem := preservation1 j (Or.inr r1) CtxRed.refl
-    apply ih lem
+  case _ _ r2 ih => apply preservation1 ih (Or.inr r2) CtxRed.refl
 
-  theorem preservation_ctx : Γ ⊢ t : A -> CtxRedStar Γ Γ' -> Γ' ⊢ t : A := by
+  theorem preservation_ctx : Γ ⊢ t : A -> @Star (Ctx Term) CtxRed Γ Γ' -> Γ' ⊢ t : A := by
   intro j r; induction r
   case _ => apply j
-  case _ r1 _r2 ih =>
-    have lem := preservation1 j (Or.inl rfl) r1
-    apply ih lem
+  case _ r2 ih => apply preservation1 ih (Or.inl rfl) r2
 
   theorem preservation_type : Γ ⊢ t : A -> A -β>* A' -> Γ ⊢ t : A' := by
   intro j r
   have lem := classification j
   cases lem
-  case _ h =>
-    subst h; cases r; apply j
-    case _ r _ => cases r
+  case _ h => sorry
+    -- subst h; cases r; apply j
+    -- case _ r _ => cases r
   case _ h =>
     cases h; case _ K h =>
       apply Judgment.conv; apply j
       apply preservation_term; apply h; apply r
-      exists A'; apply And.intro; apply r; apply Red.refl
+      exists A'; apply And.intro; apply r; apply Star.refl
 
-  theorem preservation_wf : ⊢ Γ -> CtxRedStar Γ Γ' -> ⊢ Γ' := by
+  theorem preservation_wf : ⊢ Γ -> @Star (Ctx Term) CtxRed Γ Γ' -> ⊢ Γ' := by
   intro j r
   induction r
   case _ => apply j
-  case _ r1 _r2 ih =>
-    have lem := preservation1 j r1
-    apply ih lem
+  case _ r2 ih => apply preservation1 ih r2
 
   theorem preservation :
     Γ ⊢ t : A ->
-    CtxRedStar Γ Γ' ->
+    @Star (Ctx Term) CtxRed Γ Γ' ->
     t -β>* t' ->
     A -β>* A' ->
     Γ' ⊢ t' : A'
