Common.lean
@@ -1,10 +1,6 @@
 
-import Common.Mathlib
-import Common.Term
-import Common.Term.Normal
-import Common.Term.Classify
-import Common.Term.Substitution
+
+import Common.Substitution
 import Common.Ctx
 import Common.Reduction
-import Common.Term.Erasure
 import Common.Util
