Fomega/Basic/Derivations.lean
@@ -1,6 +1,6 @@
 import Common
+import Fomega.Term
 import Fomega.Proof
-import Fomega.PreProof
 import Fomega.Basic.Weaken
 import Fomega.Basic.Substitution
 import Fomega.Basic.Inversion
@@ -9,10 +9,10 @@ import Fomega.Basic.Classification
 namespace Fomega
 
   @[simp]
-  def uid (t : Term) : Term := .unit_rec .unit t
+  def uid (t : Term) : Term := .unit_rec (u) t
 
   -- ⊢ (X : ★) -> X
   @[simp]
-  def Bot : Term := ∀f[★] 0!!
+  def Bot : Term := Π[★] #0
 
 end Fomega
