Fomega/Basic/Substitution.lean
@@ -1,42 +1,41 @@
 
 import Common
 import Fomega.Proof
-import Fomega.PreProof
 import Fomega.Basic.Weaken
 
 namespace Fomega.Proof
 
-  theorem lift_subst_rename :
-    (∀ n y, σ n = .rename y -> [σ](Γ d@ n) = Δ d@ y) ->
-    (∀ n y, ^σ n = .rename y -> [^σ]((A :: Γ) d@ n) = ([σ]A :: Δ) d@ y)
+  theorem lift_subst_rename (A : Term) :
+    (∀ n y, σ n = .re y -> [σ](Γ d@ n) = Δ d@ y) ->
+    (∀ n y, ^σ n = .re y -> [^σ]((A :: Γ) d@ n) = ([σ]A :: Δ) d@ y)
   := by
   intro h1 n y h2
   cases n
   case _ => simp at *; subst h2; simp
   case _ n =>
-    simp at *; unfold Term.Subst.compose at h2; simp at h2
+    simp at *; unfold Subst.compose at h2; simp at h2
     generalize ydef : σ n = y at *
     cases y <;> simp at h2
     case _ z =>
       subst h2; simp
       replace h1 := h1 n z ydef
-      rw [<-Term.subst_apply_compose_commute, h1]
+      rw [<-Term.apply_compose, h1]
 
   theorem lift_subst_replace :
     Δ ⊢ ([σ]A) : .const K ->
-    (∀ n t, σ n = .replace t -> Δ ⊢ t : ([σ]Γ d@ n)) ->
-    (∀ n t, ^σ n = .replace t -> ([σ]A :: Δ) ⊢ t : ([^σ](A :: Γ) d@ n))
+    (∀ n t, σ n = .su t -> Δ ⊢ t : ([σ]Γ d@ n)) ->
+    (∀ n t, ^σ n = .su t -> ([σ]A :: Δ) ⊢ t : ([^σ](A :: Γ) d@ n))
   := by
   intro j h1 n t h2
   cases n <;> simp at *
   case _ n =>
-    unfold Term.Subst.compose at h2; simp at h2
+    unfold Subst.compose at h2; simp at h2
     generalize ydef : σ n = y at *
     cases y <;> simp at h2
     case _ t' =>
       replace h1 := h1 n t' ydef
       subst h2
-      rw [<-Term.subst_apply_compose_commute]
+      rw [<-Term.apply_compose]
       apply weaken; apply j; apply h1
 
   @[simp]
@@ -46,8 +45,8 @@ namespace Fomega.Proof
     | .wf => λ () => ()
 
   theorem subst :
-    (∀ n y, σ n = .rename y -> [σ](Γ d@ n) = Δ d@ y) ->
-    (∀ n t, σ n = .replace t -> Δ ⊢ t : ([σ]Γ d@ n)) ->
+    (∀ n y, σ n = .re y -> [σ](Γ d@ n) = Δ d@ y) ->
+    (∀ n t, σ n = .su t -> Δ ⊢ t : ([σ]Γ d@ n)) ->
     Judgment v Γ idx ->
     ⊢ Δ ->
     Judgment v Δ (idx_subst σ idx)
@@ -57,30 +56,30 @@ namespace Fomega.Proof
   case nil => apply j2
   case cons => apply j2
   case ax Γ _j _ih => simp; constructor; apply j2
-  case var Γ x K T _q1 q2 ih =>
+  case var x _ h ih =>
     simp; generalize zdef : σ x = z
     cases z
     case _ y =>
-      replace ih := ih h2 h3 j2; simp at ih; rw [h2 x y zdef] at ih
-      simp; rw [q2, h2 x y zdef]
-      constructor; apply ih; rfl
-    case _ t => simp; rw [q2]; apply h3 x t zdef
+      simp at *; subst h; rw [h2 _ _ zdef]
+      constructor; apply j2; rfl
+    case _ t =>
+      simp at *; subst h; apply h3 _ _ zdef
   case pi Γ A K1 K2 B _j1 _j2 ih1 ih2 =>
     have lem1 := ih1 h2 h3 j2
     have lem2 : ⊢ ([σ]A :: Δ) := by constructor; apply j2; apply lem1
     simp; constructor; apply ih1 h2 h3 j2
-    replace ih2 := @ih2 (^σ) ([σ]A :: Δ) (lift_subst_rename h2) (lift_subst_replace lem1 h3) lem2
+    replace ih2 := @ih2 (^σ) ([σ]A :: Δ) (lift_subst_rename _ h2) (lift_subst_replace lem1 h3) lem2
     simp at ih2; exact ih2
   case lam Γ A K1 K2 B t _j1 _j2 _j3 ih1 ih2 ih3 =>
     have lem1 := ih1 h2 h3 j2
     have lem2 : ⊢ ([σ]A :: Δ) := by constructor; apply j2; apply lem1
     simp; constructor; simp at *; apply ih1 h2 h3 j2
-    replace ih2 := @ih2 (^σ) ([σ]A :: Δ) (lift_subst_rename h2)  (lift_subst_replace lem1 h3) lem2
+    replace ih2 := @ih2 (^σ) ([σ]A :: Δ) (lift_subst_rename _ h2)  (lift_subst_replace lem1 h3) lem2
     simp at ih2; exact ih2
-    replace ih3 := @ih3 (^σ) ([σ]A :: Δ) (lift_subst_rename h2)  (lift_subst_replace lem1 h3) lem2
+    replace ih3 := @ih3 (^σ) ([σ]A :: Δ) (lift_subst_rename _ h2)  (lift_subst_replace lem1 h3) lem2
     simp at ih3; exact ih3
   case app _j1 _j2 j3 ih1 ih2 =>
-    simp; constructor; apply ih1 h2 h3 j2; apply ih2 h2 h3 j2
+    simp; constructor; simp at ih1; apply ih1 h2 h3 j2; apply ih2 h2 h3 j2
     subst j3; simp
   case prod ih1 ih2 =>
     simp; constructor; apply ih1 h2 h3 j2; apply ih2 h2 h3 j2
@@ -100,11 +99,11 @@ namespace Fomega.Proof
     apply ih2 h2 h3 j2; apply ih3 h2 h3 j2
   case conv Γ' t' A' B K _j1 _j2 j3 ih1 ih2 =>
     constructor; apply ih1 h2 h3 j2; apply ih2 h2 h3 j2
-    apply RedConv.subst _ j3
+    apply Red.subst_same j3
 
   theorem beta : (A::Γ) ⊢ b : B -> Γ ⊢ t : A -> Γ ⊢ (b β[t]) : (B β[t]) := by
   simp; intro j1 j2
-  have lem := @subst (.replace t :: I) (A::Γ) Γ .prf (b, B); simp at lem
+  have lem := @subst (.su t :: I) (A::Γ) Γ .prf (b, B); simp at lem
   apply lem
   case _ =>
     intro n y h
