Fomega/Basic/Weaken.lean
@@ -1,28 +1,29 @@
 
 import Common
 import Fomega.Proof
-import Fomega.PreProof
+import Fomega.Reduction
 
 namespace Fomega.Proof
 
-  theorem rename_lift r A :
-    (∀ x, [r#r](Γ d@ x) = Δ d@ (r x)) ->
-    ∀ x, [r#(Term.Ren.lift r)]((A::Γ) d@ x) = ([r#r]A::Δ) d@ (Term.Ren.lift r x)
+  theorem rename_lift r (A : Term) :
+    (∀ x, [r.to](Γ d@ x) = Δ d@ (r x)) ->
+    ∀ x, [r.lift.to]((A::Γ) d@ x) = ([r.to]A::Δ) d@ (Ren.lift r x)
   := by
   intro h x; simp
   cases x <;> simp at *
-  case _ x => rw [<-h x]; simp
+  case _ => rw [Subst.lift_lemma]; simp
+  case _ x => rw [Subst.lift_lemma, <-h x]; simp
 
   @[simp]
   abbrev idx_ren (r : Ren) : JudgmentIndex v -> JudgmentIndex v :=
     match v with
-    | .prf => λ (t, A) => ([r#r]t, [r#r]A)
+    | .prf => λ (t, A) => ([r.to]t, [r.to]A)
     | .wf => λ () => ()
 
   theorem rename (r : Ren) :
     Judgment v Γ idx ->
     ⊢ Δ ->
-    (∀ x, [r#r](Γ d@ x) = Δ d@ (r x)) ->
+    (∀ x, [r.to](Γ d@ x) = Δ d@ (r x)) ->
     Judgment v Δ (idx_ren r idx)
   := by
   intro j h1 h2
@@ -32,30 +33,30 @@ namespace Fomega.Proof
   case ax ih =>
     replace ih := ih r h1 h2
     simp at *; constructor; apply ih
-  case var x K T _j1 j2 ih =>
-    simp at *; rw [j2, h2 x]; constructor
-    rw [<-(h2 x)]; apply ih r h1 h2; rfl
+  case var _ h _ =>
+    simp at *; constructor; apply h1; subst h
+    apply h2
   case pi Γ A K1 K2 B _j1 _j2 ih1 ih2 =>
     simp; constructor
     case _ => apply ih1 r h1 h2
     case _ =>
-      have lem : ⊢ ([r#r]A :: Δ) := by constructor; apply h1; apply ih1 r h1 h2
-      replace ih2 := @ih2 ([r#r]A :: Δ) (Term.Ren.lift r) lem (rename_lift r A h2)
-      simp at ih2; exact ih2
+      have lem : ⊢ ([r.to]A :: Δ) := by constructor; apply h1; apply ih1 r h1 h2
+      replace ih2 := @ih2 ([r.to]A :: Δ) (Ren.lift r) lem (rename_lift r A h2)
+      simp at ih2; rw [Subst.lift_lemma] at ih2; simp at ih2; exact ih2
   case lam Γ A K1 K2 B t _j1 _j2 _j3 ih1 ih2 ih3 =>
-    have lem : ⊢ ([r#r]A :: Δ) := by
+    have lem : ⊢ ([r.to]A :: Δ) := by
       constructor; apply h1; apply ih1 r h1 h2
     simp; constructor
     case _ => apply ih1 r h1 h2
     case _ =>
-      replace ih2 := @ih2 ([r#r]A :: Δ) (Term.Ren.lift r) lem (rename_lift r A h2)
-      simp at ih2; exact ih2
+      replace ih2 := @ih2 ([r.to]A :: Δ) (Ren.lift r) lem (rename_lift r A h2)
+      simp at ih2; rw [Subst.lift_lemma] at ih2; simp at ih2; exact ih2
     case _ =>
-      replace ih3 := @ih3 ([r#r]A :: Δ) (Term.Ren.lift r) lem (rename_lift r A h2)
-      simp at ih3; exact ih3
+      replace ih3 := @ih3 ([r.to]A :: Δ) (Ren.lift r) lem (rename_lift r A h2)
+      simp at ih3; rw [Subst.lift_lemma] at ih3; simp at ih3; exact ih3
   case app Γ' f A' B a B' _j1 _j2 j3 ih1 ih2 =>
     simp; constructor
-    case _ => apply ih1 r h1 h2
+    case _ => simp at ih1; apply ih1 r h1 h2
     case _ => apply ih2 r h1 h2
     case _ => subst j3; simp
   case prod ih1 ih2 =>
@@ -83,7 +84,7 @@ namespace Fomega.Proof
     constructor
     case _ => apply ih1 r h1 h2
     case _ => apply ih2 r h1 h2
-    case _ => apply RedConv.subst; apply j3
+    case _ => apply Red.subst_same; apply j3
 
   theorem weaken :
     Γ ⊢ B : .const K ->
@@ -92,6 +93,6 @@ namespace Fomega.Proof
   := by
   intro j1 j2; apply rename _ j2;
   case _ => constructor; apply judgment_ctx_wf j1; apply j1
-  case _ => intro x; simp; rw [Term.S_to_rS]; unfold rS; simp
+  case _ => intro x; simp; rw [Subst.to_S]
 
 namespace Fomega.Proof
