Fomega/PreProof.lean
@@ -1,158 +1,158 @@
 
-import Common
-import Fomega.Proof
+-- import Common
+-- import Fomega.Proof
 
-namespace Fomega
+-- namespace Fomega
 
-  theorem judgment_ctx_wf : Judgment v Γ idx -> ⊢ Γ := by
-  intro j
-  induction j
-  case nil => constructor
-  case cons j1 j2 _ _ => constructor; apply j1; apply j2
-  all_goals try simp [*]
+--   theorem judgment_ctx_wf : Judgment v Γ idx -> ⊢ Γ := by
+--   intro j
+--   induction j
+--   case nil => constructor
+--   case cons j1 j2 _ _ => constructor; apply j1; apply j2
+--   all_goals try simp [*]
 
-  inductive IsPreProof : Term -> Prop where
-  | ax : IsPreProof (.const K)
-  | bound : IsPreProof (.bound K x)
-  | all : IsPreProof A -> IsPreProof B -> IsPreProof (.all mf A B)
-  | lam : IsPreProof A -> IsPreProof t -> IsPreProof (.lam mf A t)
-  | app : IsPreProof f -> IsPreProof a -> IsPreProof (.app mf f a)
-  | times : IsPreProof A -> IsPreProof B -> IsPreProof (.times A B)
-  | pair : IsPreProof a -> IsPreProof b -> IsPreProof (.pair a b)
-  | fst : IsPreProof t -> IsPreProof (.fst t)
-  | snd : IsPreProof t -> IsPreProof (.snd t)
-  | unit_ty : IsPreProof .unit_ty
-  | unit : IsPreProof .unit
-  | unit_rec : IsPreProof t1 -> IsPreProof t2 -> IsPreProof (.unit_rec t1 t2)
+--   inductive IsPreProof : Term -> Prop where
+--   | ax : IsPreProof (.const K)
+--   | bound : IsPreProof (.bound K x)
+--   | all : IsPreProof A -> IsPreProof B -> IsPreProof (.all mf A B)
+--   | lam : IsPreProof A -> IsPreProof t -> IsPreProof (.lam mf A t)
+--   | app : IsPreProof f -> IsPreProof a -> IsPreProof (.app mf f a)
+--   | times : IsPreProof A -> IsPreProof B -> IsPreProof (.times A B)
+--   | pair : IsPreProof a -> IsPreProof b -> IsPreProof (.pair a b)
+--   | fst : IsPreProof t -> IsPreProof (.fst t)
+--   | snd : IsPreProof t -> IsPreProof (.snd t)
+--   | unit_ty : IsPreProof .unit_ty
+--   | unit : IsPreProof .unit
+--   | unit_rec : IsPreProof t1 -> IsPreProof t2 -> IsPreProof (.unit_rec t1 t2)
 
-  namespace IsPreProof
-    theorem from_subst : IsPreProof ([σ]t) -> IsPreProof t := by
-    intro j
-    induction t generalizing σ <;> (try (simp at j; cases j))
-    case bound K x => constructor
-    case _ => constructor
-    case _ ih1 ih2 j1 j2 =>
-      constructor; apply ih1 j1; apply ih2 j2
-    case _ ih1 ih2 j1 j2 =>
-      constructor; apply ih1 j1; apply ih2 j2
-    case _ ih1 ih2 j1 j2 =>
-      constructor; apply ih1 j1; apply ih2 j2
-    case _ ih1 ih2 j1 j2 =>
-      constructor; apply ih1 j1; apply ih2 j2
-    case _ ih j => constructor; apply ih j
-    case _ ih j => constructor; apply ih j
-    case _ ih1 ih2 j1 j2 =>
-      constructor; apply ih1 j1; apply ih2 j2
-    case _ => constructor
-    case _ => constructor
-    case _ ih1 ih2 j1 j2 =>
-      constructor; apply ih1 j1; apply ih2 j2
+--   namespace IsPreProof
+--     theorem from_subst : IsPreProof ([σ]t) -> IsPreProof t := by
+--     intro j
+--     induction t generalizing σ <;> (try (simp at j; cases j))
+--     case bound K x => constructor
+--     case _ => constructor
+--     case _ ih1 ih2 j1 j2 =>
+--       constructor; apply ih1 j1; apply ih2 j2
+--     case _ ih1 ih2 j1 j2 =>
+--       constructor; apply ih1 j1; apply ih2 j2
+--     case _ ih1 ih2 j1 j2 =>
+--       constructor; apply ih1 j1; apply ih2 j2
+--     case _ ih1 ih2 j1 j2 =>
+--       constructor; apply ih1 j1; apply ih2 j2
+--     case _ ih j => constructor; apply ih j
+--     case _ ih j => constructor; apply ih j
+--     case _ ih1 ih2 j1 j2 =>
+--       constructor; apply ih1 j1; apply ih2 j2
+--     case _ => constructor
+--     case _ => constructor
+--     case _ ih1 ih2 j1 j2 =>
+--       constructor; apply ih1 j1; apply ih2 j2
 
-    theorem ren : IsPreProof t -> IsPreProof ([r#r]t) := by
-    intro j
-    induction j generalizing r <;> simp
-    case ax => constructor
-    case bound => constructor
-    case all _j1 _j2 ih1 ih2 =>
-      constructor; apply ih1
-      replace ih2 := @ih2 (Term.Ren.lift r)
-      simp at ih2; exact ih2
-    case lam _j1 _j2 ih1 ih2 =>
-      constructor; apply ih1
-      replace ih2 := @ih2 (Term.Ren.lift r)
-      simp at ih2; exact ih2
-    case app _j1 _j2 ih1 ih2 =>
-      constructor; apply ih1; apply ih2
-    case times ih1 ih2 =>
-      constructor; apply ih1; apply ih2
-    case pair ih1 ih2 =>
-      constructor; apply ih1; apply ih2
-    case fst ih => constructor; apply ih
-    case snd ih => constructor; apply ih
-    case unit => constructor
-    case unit_ty => constructor
-    case unit_rec ih1 ih2 =>
-      constructor; apply ih1; apply ih2
+--     theorem ren : IsPreProof t -> IsPreProof ([r#r]t) := by
+--     intro j
+--     induction j generalizing r <;> simp
+--     case ax => constructor
+--     case bound => constructor
+--     case all _j1 _j2 ih1 ih2 =>
+--       constructor; apply ih1
+--       replace ih2 := @ih2 (Term.Ren.lift r)
+--       simp at ih2; exact ih2
+--     case lam _j1 _j2 ih1 ih2 =>
+--       constructor; apply ih1
+--       replace ih2 := @ih2 (Term.Ren.lift r)
+--       simp at ih2; exact ih2
+--     case app _j1 _j2 ih1 ih2 =>
+--       constructor; apply ih1; apply ih2
+--     case times ih1 ih2 =>
+--       constructor; apply ih1; apply ih2
+--     case pair ih1 ih2 =>
+--       constructor; apply ih1; apply ih2
+--     case fst ih => constructor; apply ih
+--     case snd ih => constructor; apply ih
+--     case unit => constructor
+--     case unit_ty => constructor
+--     case unit_rec ih1 ih2 =>
+--       constructor; apply ih1; apply ih2
 
-    theorem lift : (∀ n s, σ n = .replace s -> IsPreProof s) -> ∀ n s, ^σ n = .replace s -> IsPreProof s := by
-    intro h n s eq; simp at *
-    cases n <;> simp at eq
-    case _ n =>
-      unfold Term.Subst.compose at eq; simp at eq
-      generalize xdef : σ n = x at *
-      cases x <;> simp at *
-      case _ t =>
-        subst eq
-        replace h := h n t xdef
-        apply ren h
+--     theorem lift : (∀ n s, σ n = .replace s -> IsPreProof s) -> ∀ n s, ^σ n = .replace s -> IsPreProof s := by
+--     intro h n s eq; simp at *
+--     cases n <;> simp at eq
+--     case _ n =>
+--       unfold Term.Subst.compose at eq; simp at eq
+--       generalize xdef : σ n = x at *
+--       cases x <;> simp at *
+--       case _ t =>
+--         subst eq
+--         replace h := h n t xdef
+--         apply ren h
 
-    theorem subst : (∀ n s, σ n = .replace s -> IsPreProof s) -> IsPreProof t -> IsPreProof ([σ]t) := by
-    intro h j
-    induction j generalizing σ <;> simp
-    case ax => constructor
-    case bound K n =>
-      generalize xdef : σ n = x at *
-      cases x <;> simp
-      case _ => constructor
-      case _ t => apply h n t xdef
-    case all _j1 _j2 ih1 ih2 =>
-      constructor; apply ih1 h
-      replace ih2 := @ih2 (^σ) (lift h)
-      simp at ih2; exact ih2
-    case lam _j1 _j2 ih1 ih2 =>
-      constructor; apply ih1 h
-      replace ih2 := @ih2 (^σ) (lift h)
-      simp at ih2; exact ih2
-    case app _j1 _j2 ih1 ih2 =>
-      constructor; apply ih1 h; apply ih2 h
-    case times ih1 ih2 =>
-      constructor; apply ih1 h; apply ih2 h
-    case pair ih1 ih2 =>
-      constructor; apply ih1 h; apply ih2 h
-    case fst ih => constructor; apply ih h
-    case snd ih => constructor; apply ih h
-    case unit => constructor
-    case unit_ty => constructor
-    case unit_rec ih1 ih2 =>
-      constructor; apply ih1 h; apply ih2 h
+--     theorem subst : (∀ n s, σ n = .replace s -> IsPreProof s) -> IsPreProof t -> IsPreProof ([σ]t) := by
+--     intro h j
+--     induction j generalizing σ <;> simp
+--     case ax => constructor
+--     case bound K n =>
+--       generalize xdef : σ n = x at *
+--       cases x <;> simp
+--       case _ => constructor
+--       case _ t => apply h n t xdef
+--     case all _j1 _j2 ih1 ih2 =>
+--       constructor; apply ih1 h
+--       replace ih2 := @ih2 (^σ) (lift h)
+--       simp at ih2; exact ih2
+--     case lam _j1 _j2 ih1 ih2 =>
+--       constructor; apply ih1 h
+--       replace ih2 := @ih2 (^σ) (lift h)
+--       simp at ih2; exact ih2
+--     case app _j1 _j2 ih1 ih2 =>
+--       constructor; apply ih1 h; apply ih2 h
+--     case times ih1 ih2 =>
+--       constructor; apply ih1 h; apply ih2 h
+--     case pair ih1 ih2 =>
+--       constructor; apply ih1 h; apply ih2 h
+--     case fst ih => constructor; apply ih h
+--     case snd ih => constructor; apply ih h
+--     case unit => constructor
+--     case unit_ty => constructor
+--     case unit_rec ih1 ih2 =>
+--       constructor; apply ih1 h; apply ih2 h
 
-    theorem beta : IsPreProof b -> IsPreProof t -> IsPreProof (b β[t]) := by
-    simp; intro j1 j2
-    apply subst
-    case _ =>
-      intro n s eq
-      cases n <;> simp at *
-      subst eq; exact j2
-    case _ => exact j1
+--     theorem beta : IsPreProof b -> IsPreProof t -> IsPreProof (b β[t]) := by
+--     simp; intro j1 j2
+--     apply subst
+--     case _ =>
+--       intro n s eq
+--       cases n <;> simp at *
+--       subst eq; exact j2
+--     case _ => exact j1
 
-    @[simp]
-    abbrev FromProofType : (v : JudgmentVariant) -> JudgmentIndex v -> Prop
-    | .prf => λ (t, _) => IsPreProof t
-    | .wf => λ () => True
+--     @[simp]
+--     abbrev FromProofType : (v : JudgmentVariant) -> JudgmentIndex v -> Prop
+--     | .prf => λ (t, _) => IsPreProof t
+--     | .wf => λ () => True
 
-    theorem from_proof : Judgment v Γ ix -> FromProofType v ix := by
-    intro j; induction j <;> simp at *
-    all_goals (try (constructor <;> simp [*]))
-    case conv => simp [*]
+--     theorem from_proof : Judgment v Γ ix -> FromProofType v ix := by
+--     intro j; induction j <;> simp at *
+--     all_goals (try (constructor <;> simp [*]))
+--     case conv => simp [*]
 
-    -- theorem from_proof_type : t ⊢ Γ -> Γ ⊢ t : A -> IsPreProof A := by
-    -- intro h j; induction j
-    -- case ax => constructor
-    -- case var =>
-    --   cases h
-    --   case _ h => apply (from_proof h)
-    -- case pi => constructor
-    -- case tpi => constructor
-    -- case lam j _ _ _ => apply from_proof j
-    -- case app _j1 j2 j3 ih1 _ih2 =>
-    --   cases h
-    --   case _ h1 h2 =>
-    --     cases (ih1 h1)
-    --     case _ p1 p2 =>
-    --     subst j3; apply beta p2 (from_proof j2)
-    -- case econv j _ _ _ => apply from_proof j
-    -- case iconv j _ _ _ => apply from_proof j
+--     -- theorem from_proof_type : t ⊢ Γ -> Γ ⊢ t : A -> IsPreProof A := by
+--     -- intro h j; induction j
+--     -- case ax => constructor
+--     -- case var =>
+--     --   cases h
+--     --   case _ h => apply (from_proof h)
+--     -- case pi => constructor
+--     -- case tpi => constructor
+--     -- case lam j _ _ _ => apply from_proof j
+--     -- case app _j1 j2 j3 ih1 _ih2 =>
+--     --   cases h
+--     --   case _ h1 h2 =>
+--     --     cases (ih1 h1)
+--     --     case _ p1 p2 =>
+--     --     subst j3; apply beta p2 (from_proof j2)
+--     -- case econv j _ _ _ => apply from_proof j
+--     -- case iconv j _ _ _ => apply from_proof j
 
-  end IsPreProof
+--   end IsPreProof
 
-end Fomega
+-- end Fomega
