Fomega/Reduction.lean
@@ -1,0 +1,195 @@
+import Fomega.Term
+import Common.Reduction
+
+inductive Red : Term -> Term -> Prop where
+-- Steps
+| beta : Red ((`λ b) `@ t) (b β[t])
+| proj1 : Red ((Term.pair t s).fst) t
+| proj2 : Red ((Term.pair t s).snd) s
+| unit_rec : Red (.unit_rec (u) t) t
+-- Congruences
+| lam_congr : Red t t' -> Red (.lam t) (.lam t')
+| app_congr1 : Red f f' -> Red (.app f t) (.app f' t)
+| app_congr2 : Red t t' -> Red (.app f t) (.app f t')
+| all_congr1 : Red A A' -> Red (.all A B) (.all A' B)
+| all_congr2 : Red B B' -> Red (.all A B) (.all A B')
+| pair_congr1 : Red t t' -> Red (.pair t s) (.pair t' s)
+| pair_congr2 : Red s s' -> Red (.pair t s) (.pair t s')
+| fst_congr : Red t t' -> Red (.fst t) (.fst t')
+| snd_congr : Red t t' -> Red (.snd t) (.snd t')
+| times_congr1 : Red A A' -> Red (.times A B) (.times A' B)
+| times_congr2 : Red B B' -> Red (.times A B) (.times A B')
+| unit_rec_congr1 : Red t1 t1' -> Red (.unit_rec t1 t2) (.unit_rec t1' t2)
+| unit_rec_congr2 : Red t2 t2' -> Red (.unit_rec t1 t2) (.unit_rec t1 t2')
+
+inductive ParRed : Term -> Term -> Prop where
+-- Steps
+| beta : ParRed b b' -> ParRed t t' -> ParRed ((`λ b) `@ t) (b' β[t'])
+| proj1 : ParRed t t' -> ParRed s s' -> ParRed ((Term.pair t s).fst) t'
+| proj2 : ParRed t t' -> ParRed s s' -> ParRed ((Term.pair t s).snd) s'
+| unit_rec : ParRed t t' -> ParRed (.unit_rec (u) t) t'
+-- Congruences
+| lam_congr : ParRed t t' -> ParRed (.lam t) (.lam t')
+| app_congr : ParRed f f' -> ParRed t t' -> ParRed (.app f t) (.app f' t')
+| all_congr : ParRed A A' -> ParRed B B' -> ParRed (.all A B) (.all A' B')
+| pair_congr : ParRed t t' -> ParRed s s' -> ParRed (.pair t s) (.pair t' s')
+| fst_congr : ParRed t t' -> ParRed (.fst t) (.fst t')
+| snd_congr : ParRed t t' -> ParRed (.snd t) (.snd t')
+| times_congr : ParRed A A' -> ParRed B B' -> ParRed (.times A B) (.times A' B')
+| unit_rec_congr : ParRed t1 t1' -> ParRed t2 t2' -> ParRed (.unit_rec t1 t2) (.unit_rec t1' t2')
+| var : ParRed (.var x) (.var x)
+| const : ParRed (.const k) (.const k)
+| unit : ParRed .unit .unit
+| unit_ty : ParRed .unit_ty .unit_ty
+
+namespace Term
+  @[simp]
+  def compl : Term -> Term
+  | app (lam b) t => (compl b) β[compl t]
+  | fst (pair t _) => compl t
+  | snd (pair _ s) => compl s
+  | unit_rec (u) t => compl t
+  | lam t => lam (compl t)
+  | app f a => app (compl f) (compl a)
+  | all A B => all (compl A) (compl B)
+  | pair t s => pair (compl t) (compl s)
+  | times t1 t2 => times (compl t1) (compl t2)
+  | fst t => fst (compl t)
+  | snd t => snd (compl t)
+  | unit => unit
+  | unit_ty => unit_ty
+  | unit_rec t1 t2 => unit_rec (compl t1) (compl t2)
+  | var n => var n
+  | const K => const K
+end Term
+
+@[simp]
+instance instReductionCompletion_Term : ReductionCompletion Term ParRed where
+  compl := Term.compl
+
+infix:40 " -β> " => Red
+infix:39 " -β>* " => @Star Term Red
+infix:38 " =β= " => @Conv Term Red
+infix:40 " =β> " => ParRed
+infix:39 " =β>* " => @Star Term ParRed
+infix:38 " ≡β≡ " => @Conv Term ParRed
+
+namespace ParRed
+  theorem red_refl : t =β> t := by
+  induction t <;> constructor <;> simp [*]
+
+  theorem red_subst_same σ : s =β> t -> [σ]s =β> [σ]t := by
+  intro h; induction h generalizing σ <;> simp
+  any_goals try apply red_refl
+  any_goals try constructor <;> simp [*]
+  case _ b b' t t' _ _ ih1 ih2 =>
+    have lem : (`λ([^σ]b) `@ ([σ]t)) =β> ([^σ]b') β[[σ]t'] := by
+      apply ParRed.beta (ih1 ^σ) (ih2 _)
+    simp at lem; apply lem
+  case _ => sorry
+  case _ => sorry
+
+  theorem red_subst (σ τ : Subst Term) :
+    (∀ n t, σ n = .su t -> ∃ t', τ n = .su t' ∧ t =β> t') ->
+    (∀ n k, σ n = .re k -> τ n = .re k) ->
+    s =β> t -> [σ]s =β> [τ]t
+  := by
+  intro h1 h2 r
+  induction r generalizing σ τ <;> simp
+  case _ b b' t t' _ _ ih1 ih2 =>
+    have lem : (`λ([^σ]b) `@ ([σ]t)) =β> ([^τ]b') β[[τ]t'] := by
+      apply ParRed.beta
+      replace ih1 := ih1 (^σ) (^τ) (Subst.lift_replace red_subst_same h1) (Subst.lift_rename h2)
+      apply ih1; apply ih2 _ _ h1 h2
+    simp at lem; apply lem
+  case _ => sorry
+  case _ => sorry
+  case _ => sorry
+  case _ => sorry
+  case _ => sorry
+  case _ => sorry
+  case _ => sorry
+  case _ => sorry
+  case _ => sorry
+  case _ => sorry
+  case _ => sorry
+  case _ => sorry
+  case _ => sorry
+  case _ => sorry
+  case _ => sorry
+  -- case _ ih1 ih2 =>
+  --   apply ParRed.app; apply ih1 _ _ h1 h2; apply ih2 _ _ h1 h2
+  -- case _ _ ih =>
+  --   constructor
+  --   replace ih := ih (^σ) (^τ) (Subst.lift_replace red_subst_same h1) (Subst.lift_rename h2)
+  --   simp at ih; apply ih
+  -- case _ x =>
+  --   generalize udef : σ x = u
+  --   cases u <;> simp at *
+  --   case _ y => rw [h2 x y udef]; simp; constructor
+  --   case _ t =>
+  --     cases (h1 x t udef); case _ v lem =>
+  --       rw [lem.1]; simp; apply lem.2
+
+  theorem red_beta : b =β> b' -> t =β> t' -> b β[t] =β> b' β[t'] := by
+  intro r1 r2; apply red_subst
+  case _ =>
+    intro n s h; cases n <;> simp at *
+    case _ => subst h; apply r2
+  case _ =>
+    intro n k h; cases n <;> simp at *; simp [*]
+  case _ => apply r1
+
+  theorem triangle : t =β> s -> s =β> Term.compl t := by
+  intro h; induction h <;> simp at * <;> try (constructor <;> simp [*])
+  case _ b b' t t' r1 r2 ih1 ih2 => apply red_beta ih1 ih2
+  case _ => sorry
+  case _ => sorry
+  case _ => sorry
+  case _ a a' f f' _ r2 ih1 ih2 => sorry
+    -- cases f <;> simp at * <;> try (constructor <;> simp [*])
+    -- case _ t =>
+    --   cases f'
+    --   case _ => cases ih2
+    --   case _ => cases r2
+    --   case _ b =>
+    --     cases ih2; case _ ih2 =>
+    --       apply ParRed.beta ih2 ih1
+  case _ => sorry
+  case _ => sorry
+  case _ => sorry
+
+end ParRed
+
+instance instReductionTriangle_Term : ReductionTriangle Term ParRed where
+  triangle := ParRed.triangle
+
+namespace Red
+  theorem red1_subst_same : t -β> s -> [σ]t -β> [σ]s := by sorry
+
+  theorem to_par1 : t -β> s -> t =β> s := by sorry
+
+  theorem from_par1 : t =β> s -> t -β>* s := by sorry
+
+  theorem to_par : t -β>* s -> t =β>* s := by sorry
+
+  theorem from_par : t =β>* s -> t -β>* s := by sorry
+
+  theorem to_conv : t =β= s -> t ≡β≡ s := by sorry
+
+  theorem from_conv : t ≡β≡ s -> t =β= s := by sorry
+
+  theorem subst_same : t =β= s -> ([σ]t) =β= ([σ]s) := by sorry
+
+  theorem const_conv_implies_eq K1 K2 : (.const K1) =β= (.const K2) -> K1 = K2 := by sorry
+
+  theorem refl : t =β= t := by sorry
+
+  theorem sym : t =β= s -> s =β= t := by sorry
+
+  theorem trans : x =β= y -> y =β= z -> x =β= z := by sorry
+
+  theorem all_congr : Π[A] B =β= Π[A'] B' -> A =β= A' ∧ B =β= B' := by sorry
+
+  theorem times_congr : (A ⊗ B) =β= (A' ⊗ B') -> A =β= A' ∧ B =β= B' := by sorry
+end Red
