Fomega/Term.lean
@@ -1,0 +1,131 @@
+import Common.Substitution
+
+inductive Const : Type where
+| kind | type
+deriving Repr
+
+inductive Term : Type where
+| var : Nat -> Term
+| const : Const -> Term
+| app : Term -> Term -> Term
+| lam : Term -> Term
+| all : Term -> Term -> Term
+| pair : Term -> Term -> Term
+| fst : Term -> Term
+| snd : Term -> Term
+| times : Term -> Term -> Term
+| unit : Term
+| unit_ty : Term
+| unit_rec : Term -> Term -> Term
+deriving Repr
+
+notation "★" => Term.const Const.type
+notation "□" => Term.const Const.kind
+infixl:15 " `@ " => Term.app
+notation "`λ" t:50 => Term.lam t
+notation "Π[" A "]" t:50 => Term.all A t
+infixl:15 "⊗" => Term.times
+notation "(u)" => Term.unit
+notation "(U)" => Term.unit_ty
+prefix:max "#" => Term.var
+
+instance instInhabited_Term : Inhabited Term where
+  default := ★
+
+namespace Term
+  @[simp]
+  def smap (lf : Subst.Lift Term) (f : Nat -> Subst.Action Term) : Term -> Term
+  | var x =>
+    match f x with
+    | .re y => var y
+    | .su t => t
+  | const k => const k
+  | app t1 t2 => app (smap lf f t1) (smap lf f t2)
+  | lam t => lam (smap lf (lf f) t)
+  | all t1 t2 => all (smap lf f t1) (smap lf (lf f) t2)
+  | pair t1 t2 => pair (smap lf f t1) (smap lf f t2)
+  | fst t => fst (smap lf f t)
+  | snd t => snd (smap lf f t)
+  | times t1 t2 => times (smap lf f t1) (smap lf f t2)
+  | unit => unit
+  | unit_ty => unit_ty
+  | unit_rec t1 t2 => unit_rec (smap lf f t1) (smap lf f t2)
+end Term
+
+@[simp↓]
+instance substType_Term : SubstitutionType Term where
+  smap := Term.smap
+
+namespace Term
+  @[simp↓]
+  theorem subst_var : [σ]#x = match σ x with | .re y => #y | .su t => t := by
+  unfold Subst.apply; simp
+
+  @[simp] -- 0[s.σ ] = s
+  theorem subst_var_replace : [.su s :: σ]var 0 = s := by simp
+
+  @[simp] -- 0[s.σ ] = s
+  theorem subst_var_rename : [.re k :: σ]var 0 = var k := by simp
+
+  @[simp]
+  theorem subst_const  : [σ]const k = const k := by unfold Subst.apply; simp
+
+  @[simp]
+  theorem subst_app : [σ](app t1 t2) = app ([σ]t1) ([σ]t2) := by unfold Subst.apply; simp
+
+  @[simp]
+  theorem subst_lam : [σ](lam t) = lam ([^σ]t) := by unfold Subst.apply; simp
+
+  @[simp]
+  theorem subst_all : [σ]all t1 t2 = all ([σ]t1) ([^σ]t2) := by unfold Subst.apply; simp
+
+  @[simp]
+  theorem subst_pair : [σ]pair t1 t2 = pair ([σ]t1) ([σ]t2) := by unfold Subst.apply; simp
+
+  @[simp]
+  theorem subst_fst : [σ]fst t = fst ([σ]t) := by unfold Subst.apply; simp
+
+  @[simp]
+  theorem subst_snd : [σ]snd t = snd ([σ]t) := by unfold Subst.apply; simp
+
+  @[simp]
+  theorem subst_times : [σ]times t1 t2 = times ([σ]t1) ([σ]t2) := by unfold Subst.apply; simp
+
+  @[simp]
+  theorem subst_unit : [σ]unit = unit := by unfold Subst.apply; simp
+
+  @[simp]
+  theorem subst_unit_ty : [σ]unit_ty = unit_ty := by unfold Subst.apply; simp
+
+  @[simp]
+  theorem subst_unit_rec : [σ]unit_rec t1 t2 = unit_rec ([σ]t1) ([σ]t2) := by unfold Subst.apply; simp
+
+  theorem apply_id {t : Term} : [I]t = t := by
+  have lem : ^I = @I Term := by
+    funext; case _ x =>
+    cases x; all_goals (unfold Subst.lift; unfold I; simp)
+  induction t
+  all_goals (simp at * <;> try simp [*])
+
+  theorem apply_stable {r : Ren} {σ : Subst Term}
+    : r.to = σ -> Ren.apply r = Subst.apply σ
+  := by
+  intro h; funext; case _ x =>
+    unfold Ren.apply; simp at *
+    unfold Ren.to; simp
+    induction x generalizing r σ <;> simp at *
+    any_goals simp [*]
+    case _ x => rw [<-h]; unfold Ren.to; simp
+    any_goals
+      rw [Subst.lift_lemma, <-h]
+      unfold Ren.fro; simp
+
+  theorem apply_compose {s : Term} {σ τ : Subst Term} : [τ][σ]s = [τ ⊙ σ]s := by
+  solve_compose Term, apply_stable, s, σ, τ
+
+end Term
+
+instance substTypeLaws_Term : SubstitutionTypeLaws Term where
+  apply_id := Term.apply_id
+  apply_compose := Term.apply_compose
+  apply_stable := Term.apply_stable
